wip

crypto/bignum/Hacl.Bignum.Fproduct.fst
@@ -20,9 +20,13 @@ let copy_from_wide_pre (s:seqelem_wide) : GTot Type0 =
   (forall (i:nat). {:pattern w (Seq.index s i)} i < len ==> w (Seq.index s i) < pow2 n)
 
 
-val copy_from_wide_spec: s:seqelem_wide{copy_from_wide_pre s} -> i:nat{i <= len} ->
-  tmp:seqelem{(forall (j:nat). (j >= i /\ j < len) ==> v (Seq.index tmp j) = w (Seq.index s j))} -> Tot seqelem
-let rec copy_from_wide_spec s i tmp =
+#set-options "--z3timeout 20"
+
+val copy_from_wide_spec_: s:seqelem_wide{copy_from_wide_pre s} ->
+  i:nat{i <= len} ->
+  tmp:seqelem{(forall (j:nat). (j >= i /\ j < len) ==> v (Seq.index tmp j) = w (Seq.index s j))} ->
+  Tot (s':seqelem{(forall (j:nat). j < len ==> v (Seq.index s' j) = w (Seq.index s j))})
+let rec copy_from_wide_spec_ s i tmp =
   if i = 0 then tmp
   else (
     let i = i - 1 in
@@ -30,53 +34,131 @@ let rec copy_from_wide_spec s i tmp =
     let tmpi = wide_to_limb si in
     Math.Lemmas.modulo_lemma (w si) (pow2 n);
     let tmp' = Seq.upd tmp i tmpi in
-    copy_from_wide_spec s i tmp'
+    copy_from_wide_spec_ s i tmp'
   )
 
 
+#set-options "--z3timeout 5"
+
+val copy_from_wide_spec: s:seqelem_wide{copy_from_wide_pre s} ->
+  Tot (s':seqelem{(forall (j:nat). j < len ==> v (Seq.index s' j) = w (Seq.index s j))})
+let rec copy_from_wide_spec s =
+  let tmp = Seq.create len limb_zero in
+  copy_from_wide_spec_ s len tmp
+
+
+#set-options "--z3timeout 50"
+
 val copy_from_wide_:
   output:felem ->
-  input:felem_wide ->
+  input:felem_wide{disjoint output input} ->
   ctr:U32.t{U32.v ctr <= len} ->
   Stack unit
-    (requires (fun _ -> true))
-    (ensures (fun _ _ _ -> true))
+    (requires (fun h -> live h output /\ live h input /\ copy_from_wide_pre (as_seq h input)
+      /\ (forall (i:nat). (i >= U32.v ctr /\ i < len) ==> v (get h output i) == w (get h input i))))
+    (ensures (fun h0 _ h1 -> live h0 input /\ copy_from_wide_pre (as_seq h0 input) /\ live h1 output
+      /\ modifies_1 output h0 h1
+      /\ as_seq h1 output == copy_from_wide_spec (as_seq h0 input) ))
 let rec copy_from_wide_ output input ctr =
-  if U32 (ctr =^ 0ul) then ()
+  if U32 (ctr =^ 0ul) then (
+    let h = ST.get() in
+    assert(forall (i:nat). i < len ==> v (Seq.index (as_seq h output) i) = w (Seq.index (as_seq h input) i));
+    Seq.lemma_eq_intro (as_seq h output) (copy_from_wide_spec (as_seq h input))
+  )
   else (
     let i = U32 (ctr -^ 1ul) in
     let inputi = input.(i) in
-    output.(i) <- Wide.wide_to_limb inputi;
+    Math.Lemmas.modulo_lemma (w inputi) (pow2 n);
+    output.(i) <- wide_to_limb inputi;
     copy_from_wide_ output input i
   )
 
 
+#set-options "--z3timeout 5"
+
+val shift_spec: seqelem -> Tot seqelem
+let shift_spec s =
+  let sfirst = Seq.slice s 0 (len - 1) in
+  let slast = Seq.slice s (len-1) len in
+  Seq.append slast sfirst
+
+#set-options "--z3timeout 50"
+
 val shift_:
   output:felem ->
-  tmp:limb ->
-  ctr:U32.t ->
+  ctr:U32.t{U32.v ctr < len} ->
   Stack unit
-    (requires (fun _ -> true))
-    (ensures (fun _ _ _ -> true))
-let rec shift_ output tmp ctr =
+    (requires (fun h -> live h output))
+    (ensures (fun h0 _ h1 -> live h0 output /\ live h1 output /\ modifies_1 output h0 h1
+      /\ (forall (i:nat). (i < U32.v ctr) ==> v (get h1 output (i+1)) = v (get h0 output i))
+      /\ (forall (i:nat). (i > U32.v ctr /\ i < len) ==> get h1 output i == get h0 output i)))
+let rec shift_ output ctr =
   let open FStar.UInt32 in
-  let tmp = if (ctr =^ clen) then output.(0ul) else tmp in
-  if (ctr =^ 1ul) then output.(1ul) <- tmp
+  if (ctr =^ 0ul) then ()
   else (
     let z = output.(ctr -^ 1ul) in
-    output.((ctr %^ clen)) <- z;
-    shift_ output tmp (ctr -^ 1ul)
+    output.(ctr) <- z;
+    shift_ output (ctr -^ 1ul)
+  )
+
+#set-options "--z3timeout 50"
+
+
+val shift:
+  output:felem ->
+  Stack unit
+    (requires (fun h -> live h output))
+    (ensures (fun h0 _ h1 -> live h0 output /\ live h1 output /\ modifies_1 output h0 h1
+      /\ as_seq h1 output == shift_spec (as_seq h0 output)))
+let rec shift output =
+  let h0 = ST.get() in
+  let open FStar.UInt32 in
+  let tmp = output.(clen -^ 1ul) in
+  shift_ output (clen -^ 1ul);
+  output.(0ul) <- tmp;
+  let h = ST.get() in
+  Seq.lemma_eq_intro (as_seq h output) (shift_spec (as_seq h0 output))
+
+#set-options "--z3timeout 20 --initial_fuel 1 --max_fuel 1"
+
+open FStar.Mul
+
+let sum_scalar_multiplication_pre_ (sw:seqelem_wide) (s:seqelem) (scalar:limb) (i:nat{i <= len}) : GTot Type0 =
+  (forall (j:nat). j < i ==> w (Seq.index sw j) + (v (Seq.index s j) * v scalar) < pow2 wide_n)
+
+
+val sum_scalar_multiplication_spec:
+  sw:seqelem_wide ->
+  s:seqelem ->
+  scalar:limb ->
+  i:nat{i <= len /\ sum_scalar_multiplication_pre_ sw s scalar i} ->
+  Tot seqelem_wide
+  (decreases i)
+let rec sum_scalar_multiplication_spec sw s scalar i =
+  if i = 0 then sw
+  else (
+    let j = i - 1 in
+    let swi = Seq.index sw j in
+    let si = Seq.index s j in
+    let open Hacl.Bignum.Wide in
+    let swi' = swi +^ (mul_wide si scalar) in
+    let sw' = Seq.upd sw j swi' in
+    sum_scalar_multiplication_spec sw' s scalar j
   )
 
 
+#set-options "--z3timeout 20 --initial_fuel 1 --max_fuel 1"
+
 val sum_scalar_multiplication_:
   output:felem_wide ->
-  input:felem ->
+  input:felem{disjoint output input} ->
   s:limb ->
-  ctr:U32.t ->
+  ctr:U32.t{U32.v ctr <= len} ->
   Stack unit
-    (requires (fun _ -> true))
-    (ensures (fun _ _ _ -> true))
+    (requires (fun h -> live h output /\ live h input /\ sum_scalar_multiplication_pre_ (as_seq h output) (as_seq h input) s (U32.v ctr)))
+    (ensures (fun h0 _ h1 -> live h1 output /\ modifies_1 output h0 h1 /\ live h0 input /\ live h0 output
+      /\ sum_scalar_multiplication_pre_ (as_seq h0 output) (as_seq h0 input) s (U32.v ctr)
+      /\ (as_seq h1 output) == sum_scalar_multiplication_spec (as_seq h0 output) (as_seq h0 input) s (U32.v ctr)))
 let rec sum_scalar_multiplication_ output input s ctr =
   if U32 (ctr =^ 0ul) then ()
   else (
@@ -84,77 +166,153 @@ let rec sum_scalar_multiplication_ output input s ctr =
     let oi = output.(i) in let ii = input.(i) in
     let open Hacl.Bignum.Wide in
     output.(i) <- (oi +^ (ii *^ s));
+    let h = ST.get() in
     sum_scalar_multiplication_ output input s i
   )
 
 
+let shift_reduce_pre (s:seqelem) : GTot Type0 = reduce_pre (shift_spec s)
+
+val shift_reduce_spec: s:seqelem{shift_reduce_pre s} -> Tot (s':seqelem)
+let shift_reduce_spec s =
+  reduce_spec (shift_spec s)
+
+
+val shift_reduce: output:felem -> Stack unit
+  (requires (fun h -> live h output /\ shift_reduce_pre (as_seq h output)))
+  (ensures (fun h0 _ h1 -> live h0 output /\ live h1 output /\ modifies_1 output h0 h1
+    /\ shift_reduce_pre (as_seq h0 output)
+    /\ as_seq h1 output == shift_reduce_spec (as_seq h0 output)))
+let shift_reduce output =
+  shift output;
+  reduce output
+
+
+
+let rec mul_shift_reduce_pre (output:seqelem_wide) (input:seqelem) (input2:seqelem) (ctr:nat{ctr <= len}) : GTot Type0 (decreases ctr) =
+  if ctr > 0 then (
+    sum_scalar_multiplication_pre_ output input (Seq.index input2 (len-ctr)) len
+    /\ (let output' = sum_scalar_multiplication_spec output input (Seq.index input2 (len-ctr)) len in
+       (ctr > 1 ==> shift_reduce_pre input) /\
+         (let input'  = if ctr > 1 then shift_reduce_spec input else input in
+          mul_shift_reduce_pre output' input' input2 (ctr-1))))
+          else true
+
+
+val mul_shift_reduce_spec:
+  output:seqelem_wide ->
+  input:seqelem -> input2:seqelem ->
+  ctr:nat{ctr <= len /\ mul_shift_reduce_pre output input input2 ctr} ->
+  Tot seqelem_wide
+  (decreases ctr)
+let rec mul_shift_reduce_spec output input input2 ctr =
+  if ctr = 0 then output
+  else (
+    let i = ctr - 1 in
+    let j = len - i - 1 in
+    let input2j = Seq.index input2 j in
+    let output' = sum_scalar_multiplication_spec output input input2j len in
+    let input'  = if ctr > 1 then shift_reduce_spec input else input in
+    mul_shift_reduce_spec output' input' input2 i
+  )
+
+#set-options "--z3timeout 50 --initial_fuel 1 --max_fuel 1"
+
 val mul_shift_reduce_:
   output:felem_wide ->
-  input:felem ->
-  input2:felem ->
-  ctr:U32.t ->
+  input:felem{disjoint output input} ->
+  input2:felem{disjoint output input2 /\ disjoint input input2}  ->
+  ctr:U32.t{U32.v ctr <= len} ->
   Stack unit
-    (requires (fun _ -> true))
-    (ensures (fun _ _ _ -> true))
+    (requires (fun h -> live h output /\ live h input /\ live h input2
+      /\ mul_shift_reduce_pre (as_seq h output) (as_seq h input) (as_seq h input2) (U32.v ctr)))
+    (ensures (fun h0 _ h1 -> live h0 output /\ live h0 input /\ live h0 input2 /\ modifies_2 output input h0 h1
+      /\ live h1 output /\ live h1 input
+      /\ mul_shift_reduce_pre (as_seq h0 output) (as_seq h0 input) (as_seq h0 input2) (U32.v ctr)
+      /\ as_seq h1 output == mul_shift_reduce_spec (as_seq h0 output) (as_seq h0 input) (as_seq h0 input2) (U32.v ctr)))
 let rec mul_shift_reduce_ output input input2 ctr =
   let open FStar.UInt32 in
   if (ctr =^ 0ul) then ()
   else (
+    let h0 = ST.get() in
     let i = ctr -^ 1ul in
     let j = clen -^ 1ul -^ i in
     let input2i = input2.(j) in
     sum_scalar_multiplication_ output input input2i clen;
-    if (ctr >^ 1ul) then shift_reduce input (ctemplate j);
+    if (ctr >^ 1ul) then shift_reduce input;
     mul_shift_reduce_ output input input2 i
   )
+
+
+#set-options "--z3timeout 10 --initial_fuel 1 --max_fuel 1"
+
+let carry_wide_pre (s:seqelem_wide) (i:nat{i < len}) : GTot Type0 =
+  w (Seq.index s i) < pow2 wide_n
+  /\ (forall (j:nat). (j > i /\ j < len) ==> w (Seq.index s j) < pow2 (wide_n - 1))
+
+
+#set-options "--lax"
+
+val carry_wide_spec: s:seqelem_wide -> i:nat{i < len} -> Tot (s':seqelem_wide)
+let rec carry_wide_spec s i =
+  if i = len - 1 then s
+  else (
+    let si = Seq.index s i in
+    let sip1 = Seq.index s (i+1) in
+    let r0 = wide_to_limb si &^ ((limb_one <<^ climb_size) -^ limb_one) in
+    let open Hacl.Bignum.Wide in
+    let c = wide_to_limb (si >>^ climb_size) in
+    let s' = Seq.upd s i (limb_to_wide r0) in
+    let s'' = Seq.upd s (i+1) (sip1 +^ limb_to_wide c) in
+    carry_wide_spec s'' (i+1)
+  )
+
 
 val carry_wide_:
   t:felem_wide ->
   ctr:U32.t ->
   Stack unit
-    (requires (fun _ -> true))
-    (ensures (fun _ _ _ -> true))
+    (requires (fun h -> live h t /\ carry_wide_pre (as_seq h t) (U32.v ctr)))
+    (ensures (fun h0 _ h1 -> live h0 t /\ live h1 t /\ modifies_1 t h0 h1
+      /\ carry_wide_pre (as_seq h0 t) (U32.v ctr)
+      /\ as_seq h1 t == carry_wide_spec (as_seq h0 t) (U32.v ctr)))
 let rec carry_wide_ t ctr =
   if U32 (ctr =^ clen -^ 1ul) then ()
   else (
     let tctr = t.(ctr) in
     let tctrp1 = t.(U32 (ctr+^1ul)) in
-    let r0 = Hacl.Bignum.Wide.wide_to_limb (tctr) &^ ((one <<^ ctemplate ctr) -^ 1ul) in
+    let r0 = wide_to_limb (tctr) &^ ((limb_one <<^ climb_size) -^ limb_one) in
     let open Hacl.Bignum.Wide in
-    let c  = Hacl.Bignum.Wide.wide_to_limb (tctr >>^ ctemplate ctr) in
-    t.(ctr) <- Hacl.Bignum.Wide.limb_to_wide r0;
-    t.(U32 (ctr +^ 1ul)) <- tctrp1 +^ Hacl.Bignum.Wide.limb_to_wide c;
+    let c  = wide_to_limb (tctr >>^ climb_size) in
+    t.(ctr) <- limb_to_wide r0;
+    t.(U32 (ctr +^ 1ul)) <- tctrp1 +^ limb_to_wide c;
     carry_wide_ t (U32 (ctr +^ 1ul))
   )
 
   
 val fmul:
   output:felem ->
-  input:felem ->
-  input2:felem ->
+  input:felem{disjoint output input} ->
+  input2:felem{disjoint output input2 /\ disjoint input input2} ->
   Stack unit
-    (requires (fun _ -> true))
-    (ensures (fun _ _ _ -> true))
+    (requires (fun h -> live h output /\ live h input /\ live h input2))
+    (ensures (fun h0 _ h1 -> modifies_2 output input h0 h1 /\ live h1 output /\ live h1 input))
 let fmul output input input2 =
   push_frame();
-  let tmp = create Wide.zero clen in
-  let t   = create Wide.zero clen in
+  let tmp = create limb_zero clen in
+  let t   = create wide_zero clen in
   blit input 0ul tmp 0ul clen;
   mul_shift_reduce_ t tmp input2 clen;
   carry_wide_ t 0ul;
   reduce_wide t;
-  (* let tnm1 = t.(U32 (len -^ 1ul)) in *)
-  (* let t0   = t.(0ul) in   *)
-  (* let c = Wide.wide_to_limb (Wide (tnm1 >>^ (ctemplate (U32 (clen -^ 1ul)))) in *)
-  (* t.(U32 (clen -^ 1ul)) <- Wide (tnm1 &^ Wide.limb_to_wide ((one <<^ ctemplate (U32 (clen -^ 1ul))) &^ 1ul)); *)
-  (* t.(0ul) <- Wide (t0 +^ (c *^ nineteen)); *)
   copy_from_wide_ output t clen;
   let output0 = output.(0ul) in
   let output1 = output.(1ul) in
-  let c = output0 >>^ (ctemplate 0ul) in
-  output.(0ul) <- output0 &^ (one <<^ ctemplate (U32 (clen -^ 1ul)) -^ 1uL);
+  let c = output0 >>^ climb_size in
+  output.(0ul) <- output0 &^ ((limb_one <<^ climb_size) -^ limb_one);
   output.(1ul) <- output1 +^ c;
   pop_frame()
+
 
 val fsquare_times_:
   input:felem ->
@@ -179,7 +337,7 @@ val fsquare_times:
     (ensures (fun _ _ _ -> true))
 let fsquare_times output input count =
   push_frame();
-  let tmp = create zero clen in
+  let tmp = create limb_zero clen in
   blit input 0ul tmp 0ul clen;
   fsquare_times_ tmp count;
   blit tmp 0ul output 0ul clen;
