crypto/bignum/Hacl.Bignum.Fscalar.fst
@@ -10,31 +10,49 @@ open Hacl.Bignum.Limb
 
 module U32 = FStar.UInt32
 
+type seqelem = s:Seq.seq limb{Seq.length s = len}
+type seqelem_wide = s:Seq.seq wide{Seq.length s = len}
+
+
+val fscalar_spec: output:seqelem_wide -> input:seqelem -> s:limb -> ctr:nat{ctr <= len} -> Tot seqelem_wide (decreases ctr)
+let rec fscalar_spec output input s ctr =
+  if ctr = 0 then output
+  else (
+    let i = ctr - 1 in
+    let inputi = Seq.index input i in
+    let open Hacl.Bignum.Wide in
+    let output' = Seq.upd output i (inputi *^ s) in
+    fscalar_spec output' input s i
+  )
+
+
 val fscalar_:
   output:felem_wide ->
-  b:felem ->
+  input:felem{disjoint input output} ->
   s:limb ->
-  i:ctr ->
+  i:ctr{U32.v i <= len} ->
   Stack unit
-    (requires (fun h -> true))
-    (ensures (fun _ _ _ -> true))
+    (requires (fun h -> live h output /\ live h input))
+    (ensures (fun h0 _ h1 -> live h0 input /\ live h0 output /\ live h1 output /\ modifies_1 output h0 h1
+      /\ as_seq h1 output == fscalar_spec (as_seq h0 output) (as_seq h0 input) s (U32.v i)))
 let rec fscalar_ output b s i =
   if U32 (i =^ 0ul) then ()
   else (
     let i = U32 (i -^ 1ul) in
     let bi = b.(i) in
     let open Hacl.Bignum.Wide in
-    b.(i) <- (bi *^ s);
+    output.(i) <- (bi *^ s);
     fscalar_ output b s i
   )
 
 
 val fscalar:
   output:felem_wide ->
-  b:felem ->
+  input:felem{disjoint output input} ->
   s:limb ->
   Stack unit
-    (requires (fun h -> true))
-    (ensures  (fun h0 _ h1 -> true))
+    (requires (fun h -> live h output /\ live h input))
+    (ensures  (fun h0 _ h1 -> live h0 output /\ live h0 input /\ live h1 output /\ modifies_1 output h0 h1
+      /\ as_seq h1 output == fscalar_spec (as_seq h0 output) (as_seq h0 input) s len))
 let fscalar output b s =
   fscalar_ output b s clen
