crypto/bignum/Hacl.Bignum.Modulo.fsti
@@ -28,18 +28,18 @@ val add_zero:
       /\ as_seq h1 b == add_zero_spec (as_seq h0 b)
       /\ eval h1 b % prime = eval h0 b % prime))
 
-val shift_reduce_pre: seqelem -> GTot Type0
+(* val shift_reduce_pre: seqelem -> GTot Type0 *)
 
 
-val shift_reduced_spec: s:seqelem{shift_reduce_pre s} -> Tot seqelem
+(* val shift_reduce_spec: s:seqelem{shift_reduce_pre s} -> Tot seqelem *)
 
 
-val shift_reduce:
-  b:felem ->
-  Stack unit
-    (requires (fun h -> live h b /\ shift_reduce_pre (as_seq h b)))
-    (ensures (fun h0 _ h1 -> live h0 b /\ shift_reduce_pre (as_seq h0 b) /\ modifies_1 b h0 h1 /\ live h1 b
-      /\ as_seq h1 b == shift_reduced_spec (as_seq h0 b)))
+(* val shift_reduce: *)
+(*   b:felem -> *)
+(*   Stack unit *)
+(*     (requires (fun h -> live h b /\ shift_reduce_pre (as_seq h b))) *)
+(*     (ensures (fun h0 _ h1 -> live h0 b /\ shift_reduce_pre (as_seq h0 b) /\ modifies_1 b h0 h1 /\ live h1 b *)
+(*       /\ as_seq h1 b == shift_reduce_spec (as_seq h0 b))) *)
 
 
 val carry_top_pre: seqelem -> GTot Type0
